cedar-lean/Cedar/Frontend/CstErrorCollector.lean
@@ -307,8 +307,7 @@ public def Relation.collectErrors (e : Relation) (req : Request) (es : Entities)
          | none   => Set.singleton (Error.cstError .nameError)) ∪
         (match inEntity with
          | none    => ∅
-         | some ie => (ie.collectErrors req es).1 ∪
-                      (if ie.toAExpr?.isNone then Set.singleton (Error.cstError .translationError) else ∅))
+         | some ie => (ie.collectErrors req es).1)
   (evalres.1 ∪ errs, evalres.2)
 termination_by sizeOf e
 decreasing_by all_goals (simp_wf; omega)
